\documentclass[letterpaper,10pt]{article}

\usepackage[english]{babel}
\usepackage[utf8]{inputenc}
\usepackage{amsmath}
\usepackage{graphicx}
\usepackage[colorinlistoftodos]{todonotes}
\usepackage[top=0.5in, bottom=0.75in, left=0.9in, right=0.9in]{geometry}
\usepackage[small]{titlesec}

\newcommand{\bes}{\begin{equation*}}
\newcommand{\ben}[1]{\begin{equation}\label{#1}}
\newcommand{\ees}{\end{equation*}}
\newcommand{\be}{\begin{equation}}
\newcommand{\ee}{\end{equation}}

\titlespacing{\section}{0pt}{\parskip}{-\parskip}

\begin{document}

\begin{flushright}
{\Large Josh Bevan - HW1Q4 - CS598APK}
\end{flushright}
\vskip -0.1in
\hrule
\vskip 0.4in

\vskip 0.1in
\section*{Use induction and the result from the previous part to show
that applying the operator
$$
  D^{-1}\phi(x) :=\int_0^x \phi(y)dy
$$
$n$ times is the same as the single application of the following operator
$$
\underbrace{(D^{-1}\circ D^{-1} \circ \cdots \circ D^{-1})}_{\text{$n$ times}}\phi
= D^{-n}\phi(x) =\frac1{(n-1)!}\int_0^x (x-y)^{n-1}\phi(y)dy
$$}

Base case: For $n=1$  the proposed statement holds:
$$
\frac1{(n-1)!}\int_0^x (x-y)^{n-1}\phi(y)dy = \int_0^x \phi(y)dy
$$
$$
\frac1{(1-1)!}\int_0^x (x-y)^{1-1}\phi(y)dy = \int_0^x \phi(y)dy
$$
$$
\frac11\int_0^x 1 \, \phi(y)dy = \int_0^x \phi(y)dy
$$

Inductive step: Assume the proposed statement holds for $n$, then for $n+1$
$$
D^{-(n+1)}\phi(x) = (D^{-1} \circ D^{-n}) \phi(x) =
\int_0^x
\frac1{(n-1)!}\int_0^z (z-y)^{n-1}\phi(y) \, dy
\, dz.
$$

Examining the domain of integration we can make an appropriate change of order of integration to obtain
$$
D^{-(n+1)}\phi(x) = \frac1{(n-1)!}
\int_0^z
\int_y^x (z-y)^{n-1}\phi(y) \, dz
\, dy
$$
and then pull out $\phi(y)$ from the inner integral
$$
D^{-(n+1)}\phi(x) = \frac1{(n-1)!}
\int_0^z \phi(y)
\int_y^x (z-y)^{n-1} \, dz
\, dy.
$$

Now we can evaluate the inner integral to obtain
$$
D^{-(n+1)}\phi(x) = \frac1{(n-1)!}
\int_0^z \phi(y)
\frac1n(x-y)^n
\, dy.
$$

Rearranging yields
$$
D^{-(n+1)}\phi(x) = \frac1{n!}
\int_0^z (x-y)^n \phi(y)\, dy.
$$

and shows that the inductive hypothesis holds.

\end{document}